File.v: add fgrow and fshrink
Interesting issue comes up: when we are growing the file, we first
allocate a block, and if that succeeds, we try to write out the new
inode containing the new block address.  But this write might fail
(because the log is full), and now we can't free the block either
(because that also requires writing via the log).

One answer seems to be leave the transaction in some unspecified
active state on error, thereby effectively requiring the caller
to abort, which is what the current theorem/spec says.

Another option is to reason more precisely about available log
space.  This doesn't seem super appealing, but I suspect this is
what Adam might tell us.

src/File.v
@@ -14,6 +14,7 @@ Require Import Eqdep_dec.
 Require Import Rec.
 Require Import Pack.
 Require Import Inode.
+Require Import Balloc.
 
 Import ListNotations.
 
@@ -139,6 +140,81 @@ Module FILE.
            [[ (F' * off |-> v)%pred (FileData (sel flist' inum empty_file)) ]]
     CRASH  LOG.log_intact lxp mbase
     >} fwrite lxp xp inum off v.
+  Proof.
+    admit.
+  Qed.
+
+  Definition fgrow T lxp bxp xp inum rx : prog T :=
+    i <- INODE.iget lxp xp inum;
+    bnum <- BALLOC.alloc lxp bxp;
+    match bnum with
+    | None => rx false
+    | Some b =>
+      (* XXX currently assumes we're growing from 0 to 1;
+       * fix once Rec.v supports arrays.
+       *)
+      let i' := (i :=> "block0" := b :=> "len" := ((i :-> "len") ^+ $1)) in
+      ok <- INODE.iput lxp xp inum i';
+      If (bool_dec ok true) {
+        rx true
+      } else {
+        (* This is pretty unfortunate: we allocated a block, but we couldn't
+         * write it into the inode (presumably because the log ran out of space.
+         * The theorem/spec of fgrow says that returning false leaves an active
+         * transaction with some unspecified state, effectively requiring the
+         * caller to abort.  But this isn't always true: one could also get a
+         * false return from BALLOC.alloc returning false above, which leaves
+         * the transaction in a clean state.  Maybe we could add a three-way
+         * return value, with an "abort" value indicating such dead-end cases?
+         *)
+        rx false
+      }
+    end.
+
+  Definition fshrink T lxp bxp xp inum rx : prog T :=
+    i <- INODE.iget lxp xp inum;
+    ok <- BALLOC.free lxp bxp (i :-> "block0");
+    If (bool_dec ok true) {
+      (* XXX currently assumes we're shrinking from 1 to 0;
+       * fix once Rec.v supports arrays.
+       *)
+      let i' := (i :=> "len" := ((i :-> "len") ^- $1)) in
+      ok <- INODE.iput lxp xp inum i';
+      rx ok
+    } else {
+      rx false
+    }.
+
+  (* Note that for [fgrow_ok] and [fshrink_ok], a [false] return value
+   * indicates that the transaction could be in any active state, so
+   * the caller is effectively forced to abort.
+   *)
+  Theorem fgrow_ok : forall lxp bxp xp inum,
+    {< F mbase m flist,
+    PRE    LOG.rep lxp (ActiveTxn mbase m) *
+           [[ (F * rep xp flist)%pred m ]] *
+           [[ (inum < $ (length flist))%word ]]
+    POST:r [[ r = false]] * (exists m', LOG.rep lxp (ActiveTxn mbase m')) \/
+           [[ r = true ]] * exists m' flist', LOG.rep lxp (ActiveTxn mbase m') *
+           [[ (F * rep xp flist')%pred m ]] *
+           [[ FileLen (sel flist' inum empty_file) = FileLen (sel flist inum empty_file) + 1 ]]
+    CRASH  LOG.log_intact lxp mbase
+    >} fgrow lxp bxp xp inum.
+  Proof.
+    admit.
+  Qed.
+
+  Theorem fshrink_ok : forall lxp bxp xp inum,
+    {< F mbase m flist,
+    PRE    LOG.rep lxp (ActiveTxn mbase m) *
+           [[ (F * rep xp flist)%pred m ]] *
+           [[ (inum < $ (length flist))%word ]]
+    POST:r [[ r = false ]] * (exists m', LOG.rep lxp (ActiveTxn mbase m')) \/
+           [[ r = true ]] * exists m' flist', LOG.rep lxp (ActiveTxn mbase m') *
+           [[ (F * rep xp flist')%pred m ]] *
+           [[ FileLen (sel flist' inum empty_file) = FileLen (sel flist inum empty_file) - 1 ]]
+    CRASH  LOG.log_intact lxp mbase
+    >} fshrink lxp bxp xp inum.
   Proof.
     admit.
   Qed.
